TAPLFormalization/02-lambda/SemanticsEquivalence.lean
@@ -31,6 +31,10 @@ lemma step_preserves_bt : BooleanTerm t₁ → t₁ ~> t₂ → BooleanTerm t₂
   intro t₁_bt st
   induction st <;> cases t₁_bt <;> grind [BooleanTerm]
 
+lemma steps_preserve_bt : BooleanTerm t₁ → t₁ ~>* t₂ → BooleanTerm t₂ := by
+  intro t₁_bt sts
+  induction sts <;> grind [step_preserves_bt]
+
 lemma subst_addDepth : subst t₁ (addDepth 1 t₂) = t₂ := by
   rw [subst]
   generalize 0 = k
@@ -51,11 +55,15 @@ lemma steps_preserve_abs : .abs t ~no~>* t' → ∃ t'_b, t' = .abs t'_b := by
 
 inductive NO'.SmallStep : IndexedTerm → IndexedTerm → Prop
     | appBody : SmallStep (.app t₁ t₂) t' → SmallStep (.app (.app t₁ t₂) t₃) (.app t' t₃)
-    | appArg : FB.isNF t₁ → SmallStep t₂ t₂' → SmallStep (.app t₁ t₂) (.app t₁ t₂')
+    | appArg : FB.Neutral t₁ → SmallStep t₂ t₂' → SmallStep (.app t₁ t₂) (.app t₁ t₂')
     | appAbs : s = subst t₂ t₁ → SmallStep (.app (.abs t₁) t₂) s
 
 infix:100 " ~no'~> " => NO'.SmallStep
 infix:100 " ~no'~>* " => ReflTransGen' NO'.SmallStep
+
+lemma no_of_no' : lx ~no'~> ly → lx ~no~> ly := by
+  intro no'_st
+  induction no'_st <;> grind [NO.SmallStep]
 
 lemma soundness_ltob_single : BR lt bt → BR lz bz → bt ~> bz → lt ~no'~>* lz := by
   intro lt_r_bt lz_r_bz b_st
@@ -96,3 +104,74 @@ theorem soundness_ltob : BR lt bt → BR lz bz → bt ~>* bz → lt ~no'~>* lz :
     let l_sts' := ih lt'_r_bt' lz_r_bz
     apply ReflTransGen'.trans ?_ l_sts'
     exact soundness_ltob_single lt_r_bt lt'_r_bt' b_st
+
+def BR' (lt : IndexedTerm) (bt : Term) : Prop := ∃ lt', lt ~no'~>* lt' ∧ BR lt' bt
+
+lemma boolean_steps_to_value : BooleanTerm bt → ∃ bz, bz.IsBooleanValue ∧ bt ~>* bz := by
+  intro bt_bool
+  induction bt_bool
+  case trueV => grind [Term, Term.IsBooleanValue, ReflTransGen']
+  case falseV => grind [Term, Term.IsBooleanValue, ReflTransGen']
+  case ifThenElse c t e c_bool t_bool e_bool c_ih t_ih e_ih =>
+    let ⟨c', ⟨c'_v, c_sts⟩⟩ := c_ih
+    let ⟨t', ⟨t'_v, t_sts⟩⟩ := t_ih
+    let ⟨e', ⟨e'_v, e_sts⟩⟩ := e_ih
+    cases c'_v
+    case trueV =>
+      exists t'
+      constructor <;> try assumption
+      calc
+        _ ~>* Term.trueV.ifThenElse t e := ReflTransGen'.lift (·.ifThenElse t e) (by grind [Term.SmallStep]) c_sts
+        _ ~> t := by constructor
+        _ ~>* _ := t_sts
+    case falseV =>
+      exists e'
+      constructor <;> try assumption
+      calc
+        _ ~>* Term.falseV.ifThenElse t e := ReflTransGen'.lift (·.ifThenElse t e) (by grind [Term.SmallStep]) c_sts
+        _ ~> e := by constructor
+        _ ~>* _ := e_sts
+
+inductive IndexedTerm.IsBooleanValue : IndexedTerm → Prop
+  | cTrue : IsBooleanValue (.abs (.abs (.boundV 0)))
+  | cFalse : IsBooleanValue (.abs (.abs (.boundV 1)))
+
+lemma br'_steps_to_value : BR' lt bt → ∃ lz bz, lz.IsBooleanValue ∧ lt ~no'~>* lz ∧ BR lz bz ∧ bt ~>* bz := by
+  rintro ⟨lt', ⟨lt_sts, t_br⟩⟩
+  let t_bt := bt_of_br t_br
+  let ⟨bz, ⟨bz_v, bt_sts⟩⟩ := boolean_steps_to_value t_bt
+  let ⟨lz, z_br⟩ := br_defined (steps_preserve_bt t_bt bt_sts)
+  exists lz, bz
+  constructor
+  · cases bz_v <;> cases z_br <;> constructor
+  · constructor
+    · apply ReflTransGen'.trans lt_sts
+      exact soundness_ltob t_br z_br bt_sts
+    · constructor <;> assumption
+
+lemma no'_triangle : lx ~no~>* ly → lx ~no'~>* lz → lz.IsBooleanValue → ly ~no'~>* lz := by
+  intro lx_to_ly lx_to_lz lz_v
+  induction lx_to_lz
+  case refl lz =>
+    cases lz_v <;> cases lx_to_ly <;> try apply ReflTransGen'.refl
+    all_goals repeat (rename_i st _; cases st)
+  case tail lx lx' lz lx_to_lx' lx'_to_lz ih =>
+    cases lx_to_ly
+    case refl => exact .tail lx_to_lx' lx'_to_lz
+    case tail lx'' lx_to_lx'' lx''_to_ly =>
+      apply ih ?_ lz_v
+      let lx_no_lx' := no_of_no' lx_to_lx'
+      let lx'_eq := NO.smallStep_deterministic.mp lx_no_lx'
+      let lx''_eq := NO.smallStep_deterministic.mp lx_to_lx''
+      grind
+
+theorem soundness_ltob' : BR' lt bt → lt ~no~>* lz → ∃ bz, BR' lz bz ∧ bt ~>* bz := by
+  intro t_br' lt_to_lz
+  let ⟨lz', ⟨bz, ⟨lz'_v, ⟨lt_to_lz', ⟨z_br, bt_to_bz'⟩⟩⟩⟩⟩ := br'_steps_to_value t_br'
+  exists bz
+  constructor
+  · exists lz'
+    constructor
+    · exact no'_triangle lt_to_lz lt_to_lz' lz'_v
+    · assumption
+  · assumption
